Proved FOLD sound and added plenty of auxiliary lemmas for soundness checks.

Charge!/src/Charge/ModularFunc/ListFunc.v
@@ -1,9 +1,11 @@
 Require Import ExtLib.Core.RelDec.
 Require Import ExtLib.Data.Fun.
 Require Import ExtLib.Tactics.Consider.
+Require Import ExtLib.Tactics.
 
 Require Import MirrorCore.TypesI.
 Require Import MirrorCore.syms.SymEnv.
+Require Import MirrorCore.syms.SymSum.
 Require Import MirrorCore.Lambda.Expr.
 
 Require Import Charge.Logics.ILogic.
@@ -11,6 +13,7 @@ Require Import Charge.ModularFunc.ListType.
 Require Import Charge.ModularFunc.BaseType.
 Require Import Charge.ModularFunc.BaseFunc.
 Require Import Charge.ModularFunc.Denotation.
+Require Import Charge.ModularFunc.SemiEqDecTyp.
 
 Require Import Coq.Strings.String.
 
@@ -99,8 +102,8 @@ Section ListFuncInst.
 	Context {func : Type} {H : ListFunc typ func}.
 	Context {Heq : RelDec (@eq typ)} {HC : RelDec_Correct Heq}.
 
-    Variable Typ2_tyArr : Typ2 _ Fun.
-    Variable Typ0_tyProp : Typ0 _ Prop.
+    Context {Typ2_tyArr : Typ2 _ Fun}.
+    Context {Typ0_tyProp : Typ0 _ Prop}.
     
     Context {Typ0_tyPropOk : Typ0Ok Typ0_tyProp}.
 
@@ -152,19 +155,23 @@ Section ListFuncInst.
     			     end
     }.
 
-  Definition listD {t : typ} (l : typD (tyList t)) : list (typD t) :=
-    eq_rect _ id l _ (btList t).
-
-  Definition listD_sym {t : typ} (l :list (typD t)) : typD (tyList t) :=
-    eq_rect _ id l _ (eq_sym (btList t)).
-
   Definition nilD t := eq_rect_r id (@nil (typD t)) (btList t).
-  Definition consD t := fun_to_typ2 (fun x xs => listD_sym (cons x (@listD t xs))).
-  Definition lengthD t := fun_to_typ (fun xs => natD_sym (List.length (@listD t xs))).
-  Definition NoDupD t := fun_to_typ (fun xs => eq_rect_r id (NoDup (@listD t xs)) (typ0_cast (Typ0 := Typ0_tyProp))).
-  Definition mapD t1 t2 := fun_to_typ2 (fun f xs => @listD_sym t2 (map (typ_to_fun f) (@listD t1 xs))).
-  Definition foldD t1 t2 := fun_to_typ3 (fun f (acc : typD t1) lst => fold_right (typ_to_fun2 f) acc (@listD t2 lst)).
-  Definition zipD t1 t2 := fun_to_typ2 (fun xs ys => listD_sym (eq_rect_r list (combine (listD xs) (listD ys)) (btPair t1 t2))).
+  Definition consD t := fun_to_typ2 (fun x (xs : typD (tyList t)) => 
+    listD_sym (cons x (listD xs))).
+  Definition lengthD t := fun_to_typ (fun (xs : typD (tyList t)) => 
+    natD_sym (List.length (listD xs))).
+  Definition NoDupD t := 
+    fun_to_typ (fun (xs : typD (tyList t)) => 
+      eq_rect_r id (NoDup (listD xs)) (typ0_cast (Typ0 := Typ0_tyProp))).
+  Definition mapD t u :=
+    fun_to_typ2 (fun (f : typD (tyArr t u)) (xs : typD (tyList t)) => 
+      listD_sym (map (typ_to_fun f) (listD xs))).
+  Definition foldD t u := 
+    fun_to_typ3 (fun (f : typD (tyArr u (tyArr t t))) (acc : typD t) (lst : typD (tyList u)) => 
+      fold_right (typ_to_fun2 f) acc (listD lst)).
+  Definition zipD t u := 
+    fun_to_typ2 (fun (xs : typD (tyList t)) (ys : typD (tyList u)) => 
+      listD_sym (eq_rect_r list (combine (listD xs) (listD ys)) (btPair t u))).
 
 	 Definition list_func_symD lf :=
 		match lf as lf return match typeof_list_func lf with
@@ -222,3 +229,433 @@ Section ListOps.
     fold_right (fun x acc => mkCons t (mkConst t x) acc) (mkNil t) lst.
   
 End ListOps.
+
+Section ListFuncOk.
+  Context {typ func : Type} {RType_typ : RType typ}.
+  Context {LF: ListFunc typ func} {RSym_func : RSym func}.
+  Context {RelDec_eq : RelDec (@eq typ)}.
+  Context {BT : BaseType typ} {BTD : BaseTypeD}.
+  Context {LT : ListType typ} {LTD : ListTypeD}.
+  Context {Typ2_tyArr : Typ2 _ Fun}.
+  Context {Typ0_Prop : Typ0 _ Prop}.
+
+  Class ListFuncOk := {
+    lf_funcAsOk (f : func) (e : list_func typ) : listS f = Some e -> 
+      forall t, 
+        funcAs f t = 
+        funcAs (RSym_func := RSym_ListFunc) e t;
+    lf_fNilOk t : listS (fNil t) = Some (pNil t);
+    lf_fConsOk t : listS (fCons t) = Some (pCons t);
+    lf_fLengthOk t : listS (fLength t) = Some (pLength t);
+    lf_fNoDupOk t : listS (fNoDup t) = Some (pNoDup t);
+    lf_fMapOk t u : listS (fMap t u) = Some (pMap t u);
+    lf_fFoldOk t u : listS (fFold t u) = Some (pFold t u);
+    lf_fZipOk t u : listS (fZip t u) = Some (pZip t u)
+  }.
+
+End ListFuncOk.
+
+Implicit Arguments ListFuncOk [[LF] [RType_typ] [RSym_func] [RelDec_eq] [LT] [LTD]
+                               [Typ2_tyArr] [Typ0_Prop] [BT] [BTD]].
+                               
+Section ListFuncBaseOk.
+  Context {typ func : Type} {RType_typ : RType typ}.
+  Context {LF: ListFunc typ func} {RSym_func : RSym func}.
+  Context {RelDec_eq : RelDec (@eq typ)}.
+  Context {RelDec_eqOk : RelDec_Correct RelDec_eq}.
+  Context {BT : BaseType typ} {BTD : BaseTypeD}.
+  Context {LT : ListType typ} {LTD : ListTypeD}.
+
+  Context {Typ2_tyArr : Typ2 _ Fun}.
+  Context {Typ0_Prop : Typ0 _ Prop}.
+
+  Let tyArr : typ -> typ -> typ := @typ2 _ _ _ _.
+  
+  Global Program Instance ListFuncBaseOk : 
+  	ListFuncOk typ (RSym_func := RSym_ListFunc) (list_func typ) := {
+    lf_funcAsOk := fun _ _ _ _ => eq_refl;
+    lf_fNilOk t := eq_refl;
+    lf_fConsOk t := eq_refl;
+    lf_fLengthOk t := eq_refl;
+    lf_fNoDupOk t := eq_refl;
+    lf_fMapOk t u := eq_refl;
+    lf_fFoldOk t u := eq_refl;
+    lf_fZipOk t u := eq_refl
+  }.
+
+End ListFuncBaseOk.
+
+Section ListFuncExprOk.
+  Context {typ func : Type} `{HOK : ListFuncOk typ func}.
+  Context {HROk : RTypeOk}.
+  Context {A : Type} {RSymA : RSym A}.
+  Context {Typ2Ok_tyArr : Typ2Ok Typ2_tyArr}.
+  Context {RSym_funcOk : RSymOk RSym_func0}.
+  
+
+  Let tyArr : typ -> typ -> typ := @typ2 _ _ _ _.
+  Let tyProp : typ := @typ0 _ _ _ _.
+
+  Lemma ListFunc_typeOk (f : func) (e : list_func typ) (H : listS f = Some e) :
+    typeof_sym f = typeof_list_func e.
+  Proof.
+    destruct HOK as [H1 H2 _ _ _ _ _ _ _].
+    specialize (H1 _ _ H).
+    destruct e; simpl in *;
+    match goal with 
+      | |- typeof_sym ?f = Some ?t => 
+	 	specialize (H1 t);
+	 	simpl in H1;
+	 	unfold funcAs in H1; simpl in H1 ; rewrite type_cast_refl in H1; [|apply _];
+	    generalize dependent (symD f);
+	 	destruct (typeof_sym f); simpl; intros; [forward|]; inversion H1
+ 	end.
+  Qed.
+  
+  Lemma lf_nil_type_eq (f : func) t t' df
+    (H1 : listS f = Some (fNil t)) (H2 : funcAs f t' = Some df) :
+    t' = tyList t.
+  Proof.
+    rewrite (lf_funcAsOk _ H1) in H2.
+    unfold funcAs in H2; simpl in *.
+    forward.
+  Qed.
+
+  Lemma lf_cons_type_eq (f : func) t t' df
+    (H1 : listS f = Some (fCons t)) (H2 : funcAs f t' = Some df) :
+    t' = tyArr t (tyArr (tyList t) (tyList t)).
+  Proof.
+    rewrite (lf_funcAsOk _ H1) in H2.
+    unfold funcAs in H2; simpl in *.
+    forward.
+    rewrite <- r. reflexivity.
+  Qed.
+
+  Lemma lf_length_type_eq (f : func) t t' df
+    (H1 : listS f = Some (fLength t)) (H2 : funcAs f t' = Some df) :
+    t' = tyArr (tyList t) tyNat.
+  Proof.
+    rewrite (lf_funcAsOk _ H1) in H2.
+    unfold funcAs in H2; simpl in *.
+    forward.
+    rewrite <- r. reflexivity.
+  Qed.
+
+  Lemma lf_NoDup_type_eq (f : func) t t' df
+    (H1 : listS f = Some (fNoDup t)) (H2 : funcAs f t' = Some df) :
+    t' = tyArr (tyList t) tyProp.
+  Proof.
+    rewrite (lf_funcAsOk _ H1) in H2.
+    unfold funcAs in H2; simpl in *.
+    forward.
+    rewrite <- r. reflexivity.
+  Qed.
+
+  Lemma lf_map_type_eq (f : func) t u t' df
+    (H1 : listS f = Some (fMap t u)) (H2 : funcAs f t' = Some df) :
+    t' = tyArr (tyArr t u) (tyArr (tyList t) (tyList u)).
+  Proof.
+    rewrite (lf_funcAsOk _ H1) in H2.
+    unfold funcAs in H2; simpl in *.
+    forward.
+    rewrite <- r. reflexivity.
+  Qed.
+
+  Lemma lf_fold_func_type_eq (f : func) t u t' df
+    (H1 : listS f = Some (fFold t u)) (H2 : funcAs f t' = Some df) :
+    t' = tyArr (tyArr u (tyArr t t)) (tyArr t (tyArr (tyList u) t)).
+  Proof.
+    rewrite (lf_funcAsOk _ H1) in H2.
+    unfold funcAs in H2; simpl in *.
+    forward.
+    rewrite <- r. reflexivity.
+  Qed.
+
+  Lemma lf_fold_type_eq (e : expr typ func) tus tvs t u t' df
+    (H1 : listS e = Some (fFold t u)) (H2 : exprD' tus tvs t' e = Some df) :
+    t' = tyArr (tyArr u (tyArr t t)) (tyArr t (tyArr (tyList u) t)).
+  Proof.
+    destruct e; simpl in *; try congruence.
+    autorewrite with exprD_rw in H2; simpl in H2; forward; inv_all; subst.
+    eapply lf_fold_func_type_eq; eassumption.
+  Qed.
+
+  Lemma lf_zip_type_eq (f : func) t u t' df
+    (H1 : listS f = Some (fZip t u)) (H2 : funcAs f t' = Some df) :
+    t' = tyArr (tyList t) (tyArr (tyList u) (tyList (tyPair t u))).
+  Proof.
+    rewrite (lf_funcAsOk _ H1) in H2.
+    unfold funcAs in H2; simpl in *.
+    forward.
+    rewrite <- r. reflexivity.
+  Qed.
+
+  Existing Instance RSym_sum.
+
+  Global Program Instance ListFuncOkSumR : ListFuncOk typ ((A + func)%type) := {
+    lf_funcAsOk := 
+      fun a f H t => 
+        match a with
+          | inl b => _
+          | inr b => _
+        end;
+    lf_fNilOk t := lf_fNilOk (func := func) t;
+    lf_fConsOk t := lf_fConsOk (func := func) t;
+    lf_fLengthOk t := lf_fLengthOk (func := func) t;
+    lf_fNoDupOk t := lf_fNoDupOk (func := func) t;
+    lf_fMapOk t u := lf_fMapOk (func := func) t u;
+    lf_fFoldOk t u := lf_fFoldOk (func := func) t u;
+    lf_fZipOk t u := lf_fZipOk (func := func) t u
+  }.
+  Next Obligation.
+    apply (lf_funcAsOk (func := func)).
+    apply H.
+  Qed.
+
+  Global Program Instance ListFuncOkSumL : ListFuncOk typ ((func + A)%type) := {
+    lf_funcAsOk := 
+      fun a f H t => 
+        match a with
+          | inl b => _
+          | inr b => _
+        end;
+    lf_fNilOk t := lf_fNilOk (func := func) t;
+    lf_fConsOk t := lf_fConsOk (func := func) t;
+    lf_fLengthOk t := lf_fLengthOk (func := func) t;
+    lf_fNoDupOk t := lf_fNoDupOk (func := func) t;
+    lf_fMapOk t u := lf_fMapOk (func := func) t u;
+    lf_fFoldOk t u := lf_fFoldOk (func := func) t u;
+    lf_fZipOk t u := lf_fZipOk (func := func) t u
+  }.
+  Next Obligation.
+    apply (lf_funcAsOk (func := func)).
+    apply H.
+  Qed.
+
+End ListFuncExprOk.
+
+Section MakeListFuncSound.
+  Context {typ func : Type} `{HOK : ListFuncOk typ func}.
+  Context {HROk : RTypeOk} {Typ2_tyArrOk : Typ2Ok Typ2_tyArr}
+          {RSym_funcOk : RSymOk RSym_func0}.
+
+  Let tyArr : typ -> typ -> typ := @typ2 _ _ _ _.
+  Let tyProp : typ := @typ0 _ _ _ _.
+  
+  Lemma lf_nil_eq (t : typ) (f : func) (df : typD (tyList t))
+    (Ho : listS f = Some (pNil t))
+    (Hf : funcAs f (tyList t) = Some df) :
+    df = nilD t.
+  Proof.
+   rewrite (lf_funcAsOk _ Ho) in Hf.
+   unfold funcAs in Hf; simpl in *.
+   rewrite type_cast_refl in Hf; [|apply HROk].
+   unfold Rcast, Relim_refl in Hf.
+   inversion Hf. reflexivity.
+  Qed.
+
+  Lemma lf_cons_eq (t : typ) (f : func) (df : typD (tyArr t (tyArr (tyList t) (tyList t))))
+    (Ho : listS f = Some (pCons t))
+    (Hf : funcAs f (tyArr t (tyArr (tyList t) (tyList t))) = Some df) :
+    df = consD t.
+  Proof.
+   rewrite (lf_funcAsOk _ Ho) in Hf.
+   unfold funcAs in Hf; simpl in *.
+   rewrite type_cast_refl in Hf; [|apply HROk].
+   unfold Rcast, Relim_refl in Hf.
+   inversion Hf. reflexivity.
+  Qed.
+
+  Lemma lf_length_eq (t : typ) (f : func) (df : typD (tyArr (tyList t) tyNat))
+    (Ho : listS f = Some (pLength t))
+    (Hf : funcAs f (tyArr (tyList t) tyNat) = Some df) :
+    df = lengthD t.
+  Proof.
+   rewrite (lf_funcAsOk _ Ho) in Hf.
+   unfold funcAs in Hf; simpl in *.
+   rewrite type_cast_refl in Hf; [|apply HROk].
+   unfold Rcast, Relim_refl in Hf.
+   inversion Hf. reflexivity.
+  Qed.
+
+  Lemma lf_NoDup_eq (t : typ) (f : func) (df : typD (tyArr (tyList t) tyProp))
+    (Ho : listS f = Some (pNoDup t))
+    (Hf : funcAs f (tyArr (tyList t) tyProp) = Some df) :
+    df = NoDupD t.
+  Proof.
+   rewrite (lf_funcAsOk _ Ho) in Hf.
+   unfold funcAs in Hf; simpl in *.
+   rewrite type_cast_refl in Hf; [|apply HROk].
+   unfold Rcast, Relim_refl in Hf.
+   inversion Hf. reflexivity.
+  Qed.
+
+  Lemma lf_map_eq (t u : typ) (f : func) (df : typD (tyArr (tyArr t u) (tyArr (tyList t) (tyList u))))
+    (Ho : listS f = Some (pMap t u))
+    (Hf : funcAs f (tyArr (tyArr t u) (tyArr (tyList t) (tyList u))) = Some df) :
+    df = mapD t u.
+  Proof.
+   rewrite (lf_funcAsOk _ Ho) in Hf.
+   unfold funcAs in Hf; simpl in *.
+   rewrite type_cast_refl in Hf; [|apply HROk].
+   unfold Rcast, Relim_refl in Hf.
+   inversion Hf. reflexivity.
+  Qed.
+
+  Lemma lf_fold_func_eq (t u : typ) (f : func) (df : typD (tyArr (tyArr u (tyArr t t)) (tyArr t (tyArr (tyList u) t))))
+    (Ho : listS f = Some (pFold t u))
+    (Hf : funcAs f (tyArr (tyArr u (tyArr t t)) (tyArr t (tyArr (tyList u) t))) = Some df) :
+    df = foldD t u.
+  Proof.
+   rewrite (lf_funcAsOk _ Ho) in Hf.
+   unfold funcAs in Hf; simpl in *.
+   rewrite type_cast_refl in Hf; [|apply HROk].
+   unfold Rcast, Relim_refl in Hf.
+   inversion Hf. reflexivity.
+  Qed.
+
+  Lemma lf_fold_eq (t u : typ) tus tvs (e : expr typ func) 
+    (df : ExprI.exprT tus tvs (typD (tyArr (tyArr u (tyArr t t)) (tyArr t (tyArr (tyList u) t)))))
+    (Ho : listS e = Some (pFold t u))
+    (Hf : exprD' tus tvs (tyArr (tyArr u (tyArr t t)) (tyArr t (tyArr (tyList u) t))) e = Some df) :
+    df = fun us vs => foldD t u.
+  Proof.
+   destruct e; simpl in *; try congruence.
+   autorewrite with exprD_rw in Hf; simpl in Hf; forward; inv_all; subst.
+   erewrite <- lf_fold_func_eq; try eassumption; reflexivity.
+  Qed.
+
+  Lemma lf_zip_eq (t u : typ) (f : func) (df : typD (tyArr (tyList t) (tyArr (tyList u) (tyList (tyPair t u)))))
+    (Ho : listS f = Some (pZip t u))
+    (Hf : funcAs f (tyArr (tyList t) (tyArr (tyList u) (tyList (tyPair t u)))) = Some df) :
+    df = zipD t u.
+  Proof.
+   rewrite (lf_funcAsOk _ Ho) in Hf.
+   unfold funcAs in Hf; simpl in *.
+   rewrite type_cast_refl in Hf; [|apply HROk].
+   unfold Rcast, Relim_refl in Hf.
+   inversion Hf. reflexivity.
+  Qed.
+
+  Lemma mkNil_sound (t : typ) tus tvs :
+    exprD' tus tvs (tyList t) (mkNil t) = Some (fun _ _ => nilD t).
+  Proof.
+    unfold mkNil; simpl.
+    autorewrite with exprD_rw; simpl; forward; inv_all; subst.
+    pose proof (lf_fNilOk t) as H1.
+    pose proof (lf_funcAsOk _ H1) as H2; rewrite H2. 
+    unfold funcAs; simpl; rewrite type_cast_refl; [|apply HROk].
+    reflexivity.
+  Qed.
+
+  Lemma mkCons_sound (t : typ) (tus tvs : tenv typ) x xs
+    (dx : ExprI.exprT tus tvs (typD t)) (dxs : ExprI.exprT tus tvs (typD (tyList t)))
+    (Hx : exprD' tus tvs t x = Some dx) (Hxs : exprD' tus tvs (tyList t) xs = Some dxs) :
+    exprD' tus tvs (tyList t) (mkCons t x xs) = Some (exprT_App (exprT_App (fun _ _ => consD t) dx) dxs).
+  Proof.
+    unfold mkCons; simpl.
+    autorewrite with exprD_rw; simpl; forward; inv_all; subst.
+    rewrite (ExprTac.exprD_typeof_Some _ _ _ xs _ Hxs).
+    autorewrite with exprD_rw; simpl; forward; inv_all; subst.
+    rewrite (ExprTac.exprD_typeof_Some _ _ _ x _ Hx).
+    autorewrite with exprD_rw; simpl; forward; inv_all; subst.
+    pose proof (lf_fConsOk t) as Ho.
+    pose proof (lf_funcAsOk _ Ho) as H1.
+    rewrite H1. unfold funcAs; simpl.
+    rewrite type_cast_refl; [reflexivity | apply _].
+  Qed.
+
+  Lemma mkLength_sound (t : typ) (tus tvs : tenv typ) lst
+    (lstD : ExprI.exprT tus tvs (typD (tyList t))) 
+    (Hlst : exprD' tus tvs (tyList t) lst = Some lstD)  :
+    exprD' tus tvs tyNat (mkLength t lst) = Some (exprT_App (fun _ _ => lengthD t) lstD).
+  Proof.
+    unfold mkLength; simpl.
+    autorewrite with exprD_rw; simpl; forward; inv_all; subst.
+    rewrite (ExprTac.exprD_typeof_Some _ _ _ lst _ Hlst).
+    autorewrite with exprD_rw; simpl; forward; inv_all; subst.
+    pose proof (lf_fLengthOk t) as Ho.
+    pose proof (lf_funcAsOk _ Ho) as H1.
+    rewrite H1. unfold funcAs; simpl.
+    rewrite type_cast_refl; [reflexivity | apply _].
+  Qed.
+
+  Lemma mkNoDup_sound (t : typ) (tus tvs : tenv typ) lst
+    (lstD : ExprI.exprT tus tvs (typD (tyList t))) 
+    (Hlst : exprD' tus tvs (tyList t) lst = Some lstD)  :
+    exprD' tus tvs tyProp (mkNoDup t lst) = Some (exprT_App (fun _ _ => NoDupD t) lstD).
+  Proof.
+    unfold mkNoDup; simpl.
+    autorewrite with exprD_rw; simpl; forward; inv_all; subst.
+    rewrite (ExprTac.exprD_typeof_Some _ _ _ lst _ Hlst).
+    autorewrite with exprD_rw; simpl; forward; inv_all; subst.
+    pose proof (lf_fNoDupOk t) as Ho.
+    pose proof (lf_funcAsOk _ Ho) as H1.
+    rewrite H1. unfold funcAs; simpl.
+    rewrite type_cast_refl; [reflexivity | apply _].
+  Qed.
+
+  Lemma mkMap_sound (t u : typ) (tus tvs : tenv typ) f lst
+    (fD : ExprI.exprT tus tvs (typD (tyArr t u)))
+    (lstD : ExprI.exprT tus tvs (typD (tyList t))) 
+    (Hf : exprD' tus tvs (tyArr t u) f = Some fD) 
+    (Hlst : exprD' tus tvs (tyList t) lst = Some lstD)  :
+    exprD' tus tvs (tyList u) (mkMap t u f lst) = Some (exprT_App (exprT_App (fun _ _ => mapD t u) fD) lstD).
+  Proof.
+    unfold mkMap; simpl.
+    autorewrite with exprD_rw; simpl; forward; inv_all; subst.
+    rewrite (ExprTac.exprD_typeof_Some _ _ _ lst _ Hlst).
+    autorewrite with exprD_rw; simpl; forward; inv_all; subst.
+    rewrite (ExprTac.exprD_typeof_Some _ _ _ f _ Hf).
+    autorewrite with exprD_rw; simpl; forward; inv_all; subst.
+    pose proof (lf_fMapOk t u) as Ho.
+    pose proof (lf_funcAsOk _ Ho) as H1.
+    rewrite H1. unfold funcAs; simpl.
+    rewrite type_cast_refl; [reflexivity | apply _].
+  Qed.
+
+  Lemma mkFold_sound (t u : typ) (tus tvs : tenv typ) f acc lst
+    (fD : ExprI.exprT tus tvs (typD (tyArr u (tyArr t t))))
+    (accD : ExprI.exprT tus tvs (typD t))
+    (lstD : ExprI.exprT tus tvs (typD (tyList u))) 
+    (Hf : exprD' tus tvs (tyArr u (tyArr t t)) f = Some fD) 
+    (Hacc : exprD' tus tvs t acc = Some accD)
+    (Hlst : exprD' tus tvs (tyList u) lst = Some lstD)  :
+    exprD' tus tvs t (mkFold t u f acc lst) = Some (exprT_App (exprT_App (exprT_App (fun _ _ => foldD t u) fD) accD) lstD).
+  Proof.
+    unfold mkFold; simpl.
+    autorewrite with exprD_rw; simpl; forward; inv_all; subst.
+    rewrite (ExprTac.exprD_typeof_Some _ _ _ lst _ Hlst).
+    autorewrite with exprD_rw; simpl; forward; inv_all; subst.
+    rewrite (ExprTac.exprD_typeof_Some _ _ _ acc _ Hacc).
+    autorewrite with exprD_rw; simpl; forward; inv_all; subst.
+    rewrite (ExprTac.exprD_typeof_Some _ _ _ f _ Hf).
+    autorewrite with exprD_rw; simpl; forward; inv_all; subst.
+    pose proof (lf_fFoldOk t u) as Ho.
+    pose proof (lf_funcAsOk _ Ho) as H2.
+    rewrite H2. unfold funcAs; simpl.
+    rewrite type_cast_refl; [reflexivity | apply _].
+  Qed.
+
+  Lemma mkZip_sound (t u : typ) (tus tvs : tenv typ) xs ys
+    (xsD : ExprI.exprT tus tvs (typD (tyList t))) 
+    (ysD : ExprI.exprT tus tvs (typD (tyList u))) 
+    (Hxs : exprD' tus tvs (tyList t) xs = Some xsD) 
+    (Hys : exprD' tus tvs (tyList u) ys = Some ysD) :
+    exprD' tus tvs (tyList (tyPair t u)) (mkZip t u xs ys) = 
+      Some (exprT_App (exprT_App (fun _ _ => zipD t u) xsD) ysD).
+  Proof.
+    unfold mkZip; simpl.
+    autorewrite with exprD_rw; simpl; forward; inv_all; subst.
+    rewrite (ExprTac.exprD_typeof_Some _ _ _ ys _ Hys).
+    autorewrite with exprD_rw; simpl; forward; inv_all; subst.
+    rewrite (ExprTac.exprD_typeof_Some _ _ _ xs _ Hxs).
+    autorewrite with exprD_rw; simpl; forward; inv_all; subst.
+    pose proof (lf_fZipOk t u) as Ho.
+    pose proof (lf_funcAsOk _ Ho) as H1.
+    rewrite H1. unfold funcAs; simpl.
+    rewrite type_cast_refl; [reflexivity | apply _].
+  Qed.
+
+End MakeListFuncSound.
+
