Charge!/src/Charge/ModularFunc/ListType.v
@@ -28,7 +28,10 @@ Section ListTypeD'.
   Definition listD (t : typ) (p : typD (tyList t)) : list (typD t) :=
     eq_rect _ id p _ (btList t).
     
-  Definition listD_inv (t : typ) (p : list (typD t)) : typD (tyList t) :=
+  Definition listD_sym (t : typ) (p : list (typD t)) : typD (tyList t) :=
     eq_rect _ id p _ (eq_sym (btList t)).
     
 End ListTypeD'.  
+
+Implicit Arguments listD [[typ] [HT] [HR] [LTD] [t]].
+Implicit Arguments listD_sym [[typ] [HT] [HR] [LTD] [t]].
