Charge!/src/Charge/ModularFunc/SemiEqDecTyp.v
@@ -1,0 +1,24 @@
+Require Import MirrorCore.TypesI.
+
+Section SemiEqDecTyp.
+  Context (typ : Type) {RType_typ : RType typ}.
+
+  Class SemiEqDecTyp := {
+    semi_eq_dec_typ : forall t (a b : typD t), option bool
+  }.
+
+  Class SemiEqDecTypOk (SemEq : SemiEqDecTyp) := {
+    semi_eq_dec_typOk :
+      forall t a b,
+        match semi_eq_dec_typ t a b with
+          | Some true => a = b
+          | Some false => a <> b
+          | None => True
+        end
+  }.
+
+End SemiEqDecTyp.
+
+Implicit Arguments SemiEqDecTypOk [[typ] [RType_typ]].
+Implicit Arguments semi_eq_dec_typ [[typ] [RType_typ] [t] [SemiEqDecTyp]].
+Implicit Arguments semi_eq_dec_typOk [[typ] [RType_typ] [SemEq] [SemiEqDecTypOk]].
